Refactor store predicates.

store/client_proofs.v
@@ -29,106 +29,103 @@ Implicit Types v : val.
 
 Variable N : namespace.
 
-Definition client_state kI kR s n t : iProp :=
+Definition client_state s n t : iProp :=
   cst_ts s ↦ #n ∗
   sterm (cst_key s) ∗
-  version_auth (cst_name s) (DfracOwn 1) n t ∗
-  store_key N Init kI kR (cst_key s) (cst_ok s) (cst_name s).
+  handshake_done N (cst_key s) (cst_ok s) ∗
+  (if cst_ok s then value_auth N (cst_key s) n t else True%I).
 
-Lemma client_state_version_frag kI kR s n t :
-  client_state kI kR s n t -∗
-  version_frag (cst_name s) n t.
+Lemma client_state_frag s n t :
+  client_state s n t -∗
+  sterm (cst_key s) ∗
+  handshake_done N (cst_key s) (cst_ok s) ∗
+  if cst_ok s then value_frag N (cst_key s) n t else True%I.
 Proof.
-iIntros "(_ & _ & ? & _)".
-by iApply version_auth_frag.
+iIntros "(_ & ? & ? & ?)"; case: cst_ok => //; iFrame.
+by iApply value_auth_frag.
 Qed.
 
-Lemma client_state_store_key kI kR s n t :
-  client_state kI kR s n t -∗
-  sterm (cst_key s) ∗
-  store_key N Init kI kR (cst_key s) (cst_ok s) (cst_name s).
-Proof. by iIntros "(_ & ? & _ & ?)"; eauto. Qed.
-
-Lemma wp_client_get_ts E kI kR s n t :
-  {{{ client_state kI kR s n t }}}
+Lemma wp_client_get_ts E s n t :
+  {{{ client_state s n t }}}
     Client.get_ts (repr s) @ E
-  {{{ RET #n; client_state kI kR s n t }}}.
+  {{{ RET #n; client_state s n t }}}.
 Proof.
 rewrite /Client.get_ts.
 iIntros "%Φ (Hl & #s_kS & Hγ & state) post".
 wp_pures. wp_load. iApply "post". iModIntro. by iFrame.
 Qed.
 
-Lemma wp_client_next_ts t' E kI kR s n t :
-  {{{ client_state kI kR s n t }}}
+Lemma wp_client_next_ts t' E s n t :
+  {{{ client_state s n t }}}
     Client.next_ts (repr s) @ E
-  {{{ RET #(); client_state kI kR s (S n) t' }}}.
+  {{{ RET #(); client_state s (S n) t' }}}.
 Proof.
 iIntros "%Ψ (n_stored & #s_key & n_t & auth) post".
-iMod (version_update t' with "n_t") as "n_t".
+iAssert (|==> if cst_ok s then value_auth N (cst_key s) (S n) t' else True)%I
+  with "[auth]" as ">auth".
+{ case: cst_ok => //.
+  by iApply (value_auth_update N t'). }
 rewrite /Client.next_ts; wp_pures; wp_load; wp_store.
 iApply "post"; iFrame.
 rewrite (_ : (n + 1)%Z = (S n)%nat :> Z); last by lia.
 by iFrame.
 Qed.
 
-Lemma wp_client_get_sk E kI kR s n t :
-  {{{ client_state kI kR s n t }}}
+Lemma wp_client_get_sk E s n t :
+  {{{ client_state s n t }}}
     Client.get_sk (repr s) @ E
-  {{{ RET (repr (Spec.mkskey (cst_key s))); client_state kI kR s n t }}}.
+  {{{ RET (repr (Spec.mkskey (cst_key s))); client_state s n t }}}.
 Proof.
 rewrite /Client.get_sk.
 iIntros "%Φ ? post". wp_pures. by iApply "post".
 Qed.
 
-Lemma wp_client_send_store E kI kR c s n t t' :
+Lemma wp_client_send_store E c s n t t' :
   ↑cryptisN ⊆ E →
   channel c -∗
-  ctx N -∗
+  store_ctx N -∗
   pterm t' -∗ (* FIXME: t' does not have to be public already *)
-  {{{ client_state kI kR s n t }}}
+  {{{ client_state s n t }}}
     Client.send_store N c (repr s) t' @ E
-  {{{ RET #(); client_state kI kR s (S n) t' }}}.
+  {{{ RET #(); client_state s (S n) t' }}}.
 Proof.
 rewrite /Client.send_store.
-iIntros "% #chan_c (#? & _) #p_t' !> %Φ state post".
+iIntros "% #chan_c (_ & #? & _) #p_t' !> %Φ state post".
 wp_pures. wp_bind (Client.next_ts _).
 iApply (wp_client_next_ts t' with "state"); iIntros "!> state".
-iPoseProof (client_state_version_frag with "state") as "#frag".
 wp_pures. wp_bind (Client.get_ts _).
 iApply (wp_client_get_ts with "state"); iIntros "!> state".
 wp_pures. wp_bind (Client.get_sk _).
 iApply (wp_client_get_sk with "state"); iIntros "!> state".
-iPoseProof (client_state_store_key with "state") as "# (s_k & p_k)".
+iPoseProof (client_state_frag with "state") as "# (s_k & p_k & frag)".
 wp_pures. wp_list. wp_bind (tint _). iApply wp_tint. wp_list.
 wp_term_of_list. wp_tsenc. wp_pures.
-iApply (wp_send with "[//]"); eauto; last by iApply "post".
+iApply (wp_send with "[//] [#]"); eauto; last by iApply "post".
 iModIntro. iApply pterm_TEncIS => //.
 - by rewrite sterm_TKey.
-- iModIntro. iExists (S n), t', kI, kR, (cst_ok s), (cst_name s).
-  do 3?iSplit => //.
-  by case: cst_ok; eauto.
+- iModIntro. iExists (S n), t', (cst_ok s).
+  by do 3?iSplit => //.
 - rewrite sterm_of_list /= sterm_TInt; do ![iSplit => //].
   by iApply pterm_sterm.
 - iModIntro. iIntros "_". rewrite pterm_of_list /= pterm_TInt. iSplit => //.
   by iSplit => //.
 Qed.
 
-Lemma wp_client_ack_store E kI kR c s n t :
+Lemma wp_client_ack_store E c s n t :
   ↑cryptisN ⊆ E →
   channel c -∗
-  ctx N -∗
-  {{{ client_state kI kR s n t }}}
+  store_ctx N -∗
+  {{{ client_state s n t }}}
     Client.ack_store N c (repr s) @ E
-  {{{ RET #(); client_state kI kR s n t }}}.
+  {{{ RET #(); client_state s n t }}}.
 Proof.
-iIntros "% #chan_c (_ & #? & _) !> %Φ state post".
+iIntros "% #chan_c (_ & _ & #? & _) !> %Φ state post".
 rewrite /Client.ack_store. wp_pures.
 wp_bind (Client.get_ts _). iApply (wp_client_get_ts with "state") => //.
 iIntros "!> state". wp_pures.
 wp_bind (Client.get_sk _). iApply (wp_client_get_sk with "state") => //.
 iIntros "!> state". wp_pures.
-iPoseProof (client_state_store_key with "state") as "#[s_k ?]".
+iPoseProof (client_state_frag with "state") as "#(s_k & ?)".
 iCombine "post state" as "I". iRevert "I".
 iApply wp_sess_recv => //. iIntros "!> %m [post state] _".
 wp_pures. wp_bind (tint _). iApply wp_tint.
@@ -137,14 +134,14 @@ wp_eq_term e; wp_pures; iModIntro; last first.
 iRight. iExists _; iSplit => //. by iApply "post".
 Qed.
 
-Lemma wp_client_store E kI kR c s n t t' :
+Lemma wp_client_store E c s n t t' :
   ↑cryptisN ⊆ E →
   channel c -∗
-  ctx N -∗
+  store_ctx N -∗
   pterm t' -∗
-  {{{ client_state kI kR s n t }}}
+  {{{ client_state s n t }}}
     Client.store N c (repr s) t' @ E
-  {{{ RET #(); client_state kI kR s (S n) t' }}}.
+  {{{ RET #(); client_state s (S n) t' }}}.
 Proof.
 iIntros "% #chan_c #ctx #p_t' !> %Φ state post". rewrite /Client.store.
 wp_pures. wp_bind (Client.send_store _ _ _ _).
@@ -158,7 +155,7 @@ Lemma wp_client_connect E c kI kR dq ph T :
   ↑cryptisN ⊆ E →
   channel c -∗
   cryptis_ctx -∗
-  ctx N -∗
+  store_ctx N -∗
   pterm (TKey Enc kI) -∗
   pterm (TKey Enc kR) -∗
   {{{ ●H{dq|ph} T }}}
@@ -166,9 +163,9 @@ Lemma wp_client_connect E c kI kR dq ph T :
   {{{ s, RET (repr s);
       ●H{dq|ph} T ∗
       ⌜cst_ok s = in_honest kI kR T⌝ ∗
-      client_state kI kR s 0 (TInt 0) }}}.
+      client_state s 0 (TInt 0) }}}.
 Proof.
-iIntros "% % #chan_c #ctx (_ & _ & _ & _ & #ctx' & #key) #p_ekI #p_ekR".
+iIntros "% % #chan_c #ctx (#? & _ & _ & _ & _ & #ctx' & #?) #p_ekI #p_ekR".
 iIntros "!> %Φ hon post". rewrite /Client.connect. wp_pures.
 iCombine "hon post" as "post". iRevert "post".
 iApply wp_do_until. iIntros "!> [hon post]". wp_pures.
@@ -178,47 +175,66 @@ iApply (wp_pk_dh_init with "[] [] [] [] [] [hon]"); eauto.
 iIntros "!> %okS [hon HokS]".
 case: okS => [kS|]; wp_pures; last by iLeft; iFrame; eauto.
 wp_alloc l as "Hl". wp_pures. wp_tag. wp_bind (mkskey _). iApply wp_mkskey.
-iMod version_alloc as "[%γ cur_term]".
-wp_pures. iRight. iExists _. iSplitR; eauto.
+iMod (version_alloc (TInt 0)) as "[%γ cur_term]".
+wp_pures.
 iDestruct "HokS" as "(#s_kS & _ & #sessW & status)".
+set (ok := in_honest kI kR T).
+set (kS' := Spec.tag _ kS).
+iAssert (handshake_done N kS' ok) as "#done".
+  iExists kI, kR, kS, ph, T.
+  by do 2!iSplit => //.
+iAssert (|==> if ok then value_auth N kS' 0 (TInt 0) else True)%I
+  with "[status cur_term]" as ">key".
+{ case e_ok: ok => //.
+  iDestruct "status" as "(#p_kS & token & #session)".
+  iMod (term_meta_set _ _ γ N with "token") as "#meta"; eauto.
+  iModIntro. iExists γ. iFrame. iSplit.
+  - iIntros "!> %kt #p_kS'".
+    rewrite (pterm_TKey kt) pterm_tag sterm_tag.
+    iDestruct "p_kS'" as "[?|[_ p_kS']]"; first by iApply "p_kS".
+    by iMod (wf_key_elim with "p_kS' [//]") as "#[]".
+  - iIntros "!> %kS'' %e".
+    case/Spec.tag_inj: e => _ <- {kS''}.
+    iExists kI, kR, ph, T. by eauto. }
+iAssert (if ok then value_frag N kS' 0 (TInt 0) else True)%I as "#frag".
+  case: ok => //.
+  by iApply value_auth_frag.
+wp_tsenc. wp_bind (send _ _).
+iApply (wp_send with "[#] [#]") => //.
+  iModIntro. iApply pterm_TEncIS => //.
+  - by rewrite sterm_TKey sterm_tag.
+  - iModIntro. iExists ok.
+    by iSplit => //.
+  - by rewrite sterm_TInt.
+  - iIntros "!> _". by rewrite pterm_TInt.
+wp_pures. iRight. iExists _. iSplitR; eauto.
 iApply ("post" $! {| cst_ts := l; cst_key := Spec.tag (N.@"key") kS;
-                     cst_name := γ;
-                     cst_ok := in_honest kI kR T |}).
+                     cst_ok := ok |}).
 rewrite /client_state /=. iFrame. rewrite sterm_tag.
 do 2!iSplitR => //.
-iExists kS, ph, T. do 3!iSplitR => //.
-case: in_honest; last by eauto.
-iDestruct "status" as "(#p_kS & token & #session)".
-iMod (term_meta_set _ _ γ N with "token") as "#meta"; eauto.
-iModIntro. do 2!iSplit => //. iIntros "!> %kt #p_kS'".
-rewrite (pterm_TKey kt) pterm_tag sterm_tag.
-iDestruct "p_kS'" as "[?|[_ p_kS']]"; first by iApply "p_kS".
-by iMod (wf_key_elim with "p_kS' key") as "#[]".
 Qed.
 
-Lemma wp_client_load E c kI kR s n t :
+Lemma wp_client_load E c s n t :
   ↑N ⊆ E →
   ↑cryptisN ⊆ E →
   channel c -∗
-  ctx N -∗
-  pterm (TKey Enc kI) -∗
-  pterm (TKey Enc kR) -∗
-  {{{ client_state kI kR s n t }}}
+  store_ctx N -∗
+  {{{ client_state s n t }}}
     Client.load N c (repr s) @ E
   {{{ t', RET (repr t');
-      client_state kI kR s n t ∗
+      client_state s n t ∗
       ◇ ⌜cst_ok s → t' = t⌝ }}}.
 Proof.
-iIntros "% % #chan_c #ctx #p_ekI #p_ekR !> %Φ state post".
+iIntros "% % #chan_c #ctx !> %Φ state post".
 rewrite /Client.load. wp_pures.
 wp_bind (Client.get_ts _). iApply (wp_client_get_ts with "state").
 iIntros "!> state". wp_pures. wp_bind (tint _). iApply wp_tint.
 wp_pures. wp_bind (Client.get_sk _).
 iApply (wp_client_get_sk with "state"). iIntros "!> state". wp_pures.
 wp_tsenc. wp_pures.
-iPoseProof (client_state_store_key with "state") as "#[s_k status]".
+iPoseProof (client_state_frag with "state") as "#(s_k & done & frag)".
 wp_bind (send _ _). iApply wp_send; eauto.
-  iDestruct "ctx" as "(_ & _ & ? & _)".
+  iDestruct "ctx" as "(_ & _ & _ & ? & _)".
   iModIntro. iApply pterm_TEncIS; eauto.
   - by rewrite sterm_TKey.
   - by rewrite sterm_TInt.
@@ -232,12 +248,11 @@ wp_eq_term e; wp_pures; last by iLeft; iFrame.
 subst n'. iModIntro. iRight. iExists _; iSplit; eauto.
 iApply ("post" $! v). iSplit => //.
 case e_ok: (cst_ok s) => //=. iIntros "_".
-iPoseProof "status"
-  as "(%kS' & %ph & %T & %e_kS & #hon & #sess & #meta & #? & #p_kS)".
-iDestruct (ack_loadE with "status ctx p_t'") as "[_ >frag]".
+iAssert (∃ γ, wf_key N (cst_key s) γ)%I as "#status".
+  by iDestruct "frag" as "(% & _ & ?)"; eauto.
+iDestruct (ack_loadE with "done status ctx p_t'") as "[_ frag']".
 iDestruct "state" as "(_ & _ & auth & _)".
-iModIntro.
-iPoseProof (version_auth_frag_agree with "auth frag") as "%e".
+iPoseProof (value_frag_agree with "done frag frag'") as ">->".
 by eauto.
 Qed.
 
